################################################################################################################################################
# Ligt (pronounce as /liXt/ or /li:t/) is a LLOD-native vocabulary for represeting Interlinear Glossed Text as RDF data                        #
# Ligt was started within the BMBF-funded Research Group "Linked Open Dictionaries (LiODi)" (2015-2020) at the Goethe Universit√§t Frankfurt #
# under the supervision of Prof. Dr. Christian Chiarcos and Dr. des. Monika Rind-Pawlowski                                                     #
# Ligt aims to provide a middle ground between LLOD vocabularies developed for other types of language resources (e.g., NIF, lemon), and       #
# several popular legacy datamodels used to represent IGT data, most notably Toolbox, FLex and Xigt.                                           #
################################################################################################################################################

#
# Ligt 0.3 core vocabulary
#

# history
# 2023-12-11 ligt 0.3: removing NIF dependency; additional optional properties introduced for versatility: ligt:utterance, ligt:correspondsTo
# 2019 09-20 [draft] Further development of sets of single examples modeling. Validation on APiCS and MSU fieldwork elicitations (MI)
# 2019-03-25 TTL+unicode validation (CC)
# 2018-01-12 introduction of ligt:UtteranceSet; now not only coherent texts can be modeled (MI)
# 2017-03-25 ligt:Document *rdfs:subClassOf* ligt:Element (CC)
# 2017-03-18 ligt 0.1: initial RDFS formalization (CC)

# contributors
# CC - Christian Chiarcos, christian.chiarcos@web.de
# MI - Max Ionov, max.ionov@gmail.com


PREFIX rdf: <http://www.w3.org/1999/02/22-rdf-syntax-ns#>
PREFIX ligt: <http://purl.org/ligt/ligt-0.3#>
PREFIX owl: <http://www.w3.org/2002/07/owl#>
PREFIX rdfs: <http://www.w3.org/2000/01/rdf-schema#>
PREFIX nif: <http://persistence.uni-leipzig.org/nlp2rdf/ontologies/nif-core#>
PREFIX oa: <http://www.w3.org/ns/oa#>
PREFIX dc: <http://purl.org/dc/terms/>

#######################
# core specifications #
#######################

ligt:Element a rdfs:Class;
	rdfs:comment "Top-level concept for Ligt classes. Introduced to define the domain of ligt:metadata."@en.

ligt:Document rdfs:subClassOf ligt:Element;
	rdfs:comment "ligt:Document corresponds to root nodes in FLex and Xigt, i.e. flex:document and xigt:xigt-corpus"@en.

ligt:hasText a owl:ObjectProperty;
	rdfs:domain ligt:Document;
	rdfs:range ligt:InterlinearText;
	rdfs:comment "ligt:hasText assignes a ligt:Document one or multiple texts."@en.

ligt:hasUtterances a owl:ObjectProperty;
	rdfs:domain ligt:Document;
	rdfs:range ligt:InterlinearCollection;
	rdfs:comment "ligt:hasUtterance assigns a ligt:Document one or more utterances. This allows representing isolated examples (e.g. APiCS or ODIN database)"@en.

ligt:InterlinearText a rdfs:Class;
    rdfs:subClassOf ligt:Segment;
    rdfs:comment "A text represents a coherent assemblage of (mostly) consecutive utterances between which meaning relations can be established. In this function, ligt:InterlinearText corresponds to flex:interlinear-text. No Xigt counterpart because Xigt has not been designed for annotating full documents but rather isolated examples harvested from the literature. In these cases, ligt:Document is linked to ligt:UtteranceGroup."@en.

ligt:InterlinearCollection a rdfs:Class;
	rdfs:subClassOf ligt:Segment;
	rdfs:comment "A collection represents a group of separate, usually non-consecutive utterances (ligt:Utterance) not linked to each by meaning. They can be a set of examples demonstrating some grammatical phenomenon, a collection of elicitations, or even a full database, e.g. APiCS. No Xigt counterpart although they are parallel to a list of all xigt:igt. No FLEx counterpart because FLEx has been designed for annotating coherent texts"@en.
	# TODO: probably, it should not be a subClassOf ligt:Segemtn because I don't think it should be segemented into paragraphs. On the other hand, segmentation of InterlinearCollection is handy. (MI)
	# TODO: check the last sentence, maybe it's not always true (MI)

ligt:Segment rdfs:subClassOf ligt:Element;
    rdfs:comment "Segment is a generalization over text-structural units at and above the level of individual glossed examples (utterances). In Toolbox, such elements can be added as free text (albeit no standard formalism exists). In FLex, these are flex:interlinear-text, flex:paragraph and flex:phrase."@en;
	rdfs:comment """Note that our use of the term follows use of "segment" follows ISO 24612:2012 (https://www.iso.org/standard/37326.html, public description under https://www.cs.vassar.edu/~ide/papers/JNLE-rev.pdf). There is no direct relation with the term "phonological segment" as used in linguistic theory."""@en.
	
ligt:hasSubSegment a owl:ObjectProperty;
    rdfs:range ligt:Segment;
	rdfs:domain ligt:Segment;
	rdfs:comment "Hierarchical relations between text segments."@en.
	
ligt:nextSegment a owl:ObjectProperty;
	rdfs:range ligt:Segment;
	rdfs:domain ligt:Segment;
	rdfs:comment "ligt:nextSegment should only hold between segments of the same type, or on the same hierarchy level, cf. ./following-sibling::*[1] in XPath. For ligt:InterlinearCollection may be omitted."@en.
	
ligt:Paragraph a rdfs:Class;
    rdfs:subClassOf ligt:Segment;
    rdfs:comment "In written text, a paragraph represents a unit of text not divided by manual line breaks. In other modalities, a paragraph can be defined as a group of utterances in discourse that are thematically closely related, e.g., sharing the same theme or topic. ligt:Paragraph is derived from flex:Paragraph."@en.

ligt:Utterance a rdfs:Class;
    rdfs:subClassOf ligt:Segment;
	rdfs:comment "A ligt:Utterance represents a single glossed example, often a sentence or a sentential fragment. We regard utterances as atomic, i.e., an utterance should not contain other utterances. ligt:Utterance corresponds to flex:phrase and xigt:igt. We avoid the term `phrase' here because it is ambiguous with `phrase' in the sense of `phrasal node' in syntax annotation (this seems to be the meaning of nif:Phrase)."@en;
	rdfs:comment "TODO: prohibit ligt:subSegment for ligt:Utterance".

ligt:hasTier a owl:ObjectProperty;
	rdfs:domain ligt:Utterance;
	rdfs:range ligt:Tier;
	rdfs:comment "introduced to connect utterances with tiers (akin to igts in Xigt)."@en.

ligt:Analysis rdfs:subClassOf ligt:Element;
	rdfs:comment "Added as a generalization over ligt:Tier and ligt:Item (whose properties represent actual annotations) to define the domain of ligt:annotation."@en.
	
ligt:Tier a rdfs:Class;
	rdfs:subClassOf ligt:Analysis;
	rdfs:comment "A tier represents a layer of annotation. ligt:Tiers, however, can also represent bundles of annotations that refer to the same segment. In this sense (and different from Xigt), a ligt:Tier represents a segmented view on a ligt:Utterance. Note that normally, multiple Xigt tiers constitute a single ligt:Tier."@en;
	rdfs:comment "TODO: at most one hasWords"@en.

ligt:WordTier rdfs:subClassOf ligt:Tier;
	rdfs:comment "A tier comprising word-level segments and their annotations. This tier is motivated by the special status of words in FLex."@en.
	
ligt:hasWords a owl:ObjectProperty;
	rdfs:subPropertyOf ligt:hasTier;
	rdfs:range ligt:WordTier.
	
ligt:hasMorphs a owl:ObjectProperty;
	rdfs:subPropertyOf ligt:hasTier;
	rdfs:range ligt:MorphTier.
	
ligt:item a owl:ObjectProperty;
	rdfs:domain ligt:Tier;
	rdfs:range ligt:Item.
	
ligt:Item a rdf:Class;
	rdfs:subClassOf ligt:Analysis;
	rdfs:comment "An item is an annotated unit in an IGT tier. The concept is grounded in Xigt, but unlike xigt:items, one ligt:Item may have multiple different annotations, then represented by annotation-specific properties."@en.

ligt:correspondsTo a owl:ObjectProperty;
	rdfs:domain ligt:Item;
	rdf:range ligt:Item.
	rdfs:comment "Establishes an alignment between two items. Normally, they should be on different tiers. However, we do not have a way to enforce this. Symmetric property."@en.
	
ligt:next a owl:ObjectProperty;
	rdfs:range ligt:Item;
	rdfs:domain ligt:Item;
	rdfs:comment "Normally, a next property should only hold between elements of one tier. However, we do not have a way to enforce this."@en.

ligt:nextMorph rdfs:subPropertyOf ligt:next;
	a owl:ObjectProperty;
	rdfs:range ligt:Morph;
	rdfs:domain ligt:Morph.

ligt:nextWord rdfs:subPropertyOf ligt:next;
	a owl:ObjectProperty;
	rdfs:range ligt:Word;
	rdfs:domain ligt:Word.
	
ligt:Word rdfs:subClassOf ligt:Item;
	rdfs:comment "A word is an orthographic correlate of minimal units of lexical or grammatical analysis in their respective syntactic context. ligt:Word is grounded in flex:Word."@en;
	rdfs:comment "ligt:Word rdfs:subClassOf some ligt:WordTier ligt:item".
	
ligt:Morph rdfs:subClassOf ligt:Item;
	rdfs:comment "A morph is a segment of a word that represents the smallest distinguishable meaningful unit, i.e., it represents the concrete instantiation of a morpheme. ligt:Morph is grounded on flex:morph."@en.
	
ligt:MorphTier rdfs:subClassOf ligt:Tier;
	rdfs:comment "A tier of morphs, motivated by the special status of morphs in FLex."@en.
	
ligt:Prefix rdfs:subClassOf ligt:Morph;
	rdfs:comment "Added in conformance with FLex."@en.
	
ligt:Stem rdfs:subClassOf ligt:Morph;
	rdfs:comment "Added in conformance with FLex."@en.

ligt:Suffix rdfs:subClassOf ligt:Morph;
	rdfs:comment "Added in conformance with FLex."@en.

ligt:Enclitic rdfs:subClassOf ligt:Morph;
	rdfs:comment "Added in conformance with FLex."@en.
	
ligt:annotation a owl:DatatypeProperty;
	rdfs:comment """ligt:annotation represents literal values assigned as annotations to items or tiers, annotations assigned to ligt:Segments are represented as ligt:metadata. This property should not be directly used, instead define subproperties detailing the kind of annotation.
	Note that we do *not* support annotating ObjectProperties as these are no core functionality of IGTs and absent from FLex, Tool and Xigt core. Where these occur (e.g., in Xigt extensions), use additional properties beyond the ligt namespace."""@en;
	rdfs:domain ligt:Analysis.
	
ligt:metadata a owl:DatatypeProperty;
	rdfs:comment """Properties that express additional information about any kind of ligt:Element, without being limited to ligt:Item or ligt:Tier, are to be implemented by subproperties of ligt:metadata and ligt:metadataRef.
	Ligt supports both literal and object metadata, with two properties ligt:metadata (cf. flex:comment) and ligt:metadataRef (cf. xigt:ref).	
	We do not prescribe what kind of literals we expect as values. The current Xigt converter produces rdf:XMLLiterals, the FLex converter produces untyped literals."""@en;
	rdfs:domain ligt:Element.
	
ligt:metadataRef a owl:ObjectProperty;
	rdfs:comment """Properties that express additional information about any kind of ligt:Element, without being limited to ligt:Item or ligt:Tier, are to be implemented by subproperties of ligt:metadata and ligt:metadataRef.
	Ligt supports both literal and object metadata, with two properties ligt:metadata (cf. flex:comment) and ligt:metadataRef (cf. xigt:ref)."""@en;
	rdfs:domain ligt:Element.
	
ligt:Metadata a rdfs:Class;
	rdfs:comment "ligt:Metadata is used for representing reified ligt:metadata, resp. ligt:metadataRef statements, with literal values being represented by ligt:metaBody, and object references by ligt:refBody. ligt:Metadata and its properties follow the Open Annotation/Web Annotation model."@en.
	
ligt:metaTarget a owl:ObjectProperty;
	rdfs:comment "Representing the *source* of a reified ligt:metadataRef or ligt:metadata annotation. Grounded on oa:hasTarget, hence the counterintuitive terminology."@en;
	rdfs:domain ligt:Metadata;
	rdfs:range ligt:Element.
	
ligt:metaBody a owl:DatatypeProperty;
	rdfs:comment "Representing the target of a reified ligt:metadata annotation. Grounded on oa:hasBody."@en;
	rdfs:domain ligt:Metadata.

ligt:refBody a owl:ObjectProperty;
	rdfs:comment "Representing the target of a reified ligt:metadataRef annotation. Grounded on oa:hasBody."@en;
	rdfs:domain ligt:Metadata.

##########################
# recommended vocabulary #
##########################

# We expect using skos:prefLabel or rdfs:label for representing the literal values
# 
	
##################################
# links to external vocabularies #
# (commented)                    #
##################################

# Dublin Core
#############

ligt:Document rdfs:subClassOf dc:Dataset.
ligt:InterlinearCollection rdfs:subClassOf dc:Dataset.
ligt:hasText rdfs:subPropertyOf dc:hasPart.
ligt:hasUtterances rdfs:subPropertyOf dc:hasPart.
ligt:InterlinearText rdfs:subClassOf dc:Text.

# NLP Interchange Format
# (http://persistence.uni-leipzig.org/nlp2rdf/ontologies/nif-core/nif-core.html)
################################################################################

# Subclassing from NIF is no longer a part of the vocabulary due to 

# Open Annotation / Web Annotation
# (https://www.w3.org/TR/annotation-vocab/)
###########################################

ligt:Metadata rdfs:subClassOf oa:Annotation.
ligt:metaTarget rdfs:subPropertyOf oa:hasTarget.
ligt:metaBody rdfs:subPropertyOf oa:hasBody.
ligt:refBody rdfs:subPropertyOf oa:hasBody.

##############################
# Remarks, open issues, etc. #
##############################

# to check: modeling tiers as rdf:Collection?
